Tactic rforward working on all examples so far May not work on symbolic execution with a residue closes #12

mc_reify/symexe_soundness.v
@@ -12,12 +12,10 @@ Require Import mc_reify.funcs.
 Require Import mc_reify.func_defs.
 Require Import mc_reify.app_lemmas.
 
-Locate THEN.
-
 
 Section tbled.
 
-Parameter tbl : SymEnv.functions RType_typ.
+Variable tbl : SymEnv.functions RType_typ.
 
 Let RSym_sym := RSym_sym tbl.
 Existing Instance RSym_sym.
@@ -29,7 +27,7 @@ Existing Instance Expr_expr_fs.
 Let Expr_ok_fs := Expr_ok_fs tbl.
 Existing Instance Expr_ok_fs.
 
-Let ExprVar_expr := @ExprVariables.ExprVar_expr.
+Let ExprVar_expr := @ExprVariables.ExprVar_expr typ func.
 Existing Instance ExprVar_expr.
 
 Existing Instance MA.
@@ -49,7 +47,12 @@ apply INSTANTIATE_sound.
 apply runOnGoals_sound. auto.
 Qed.
 
-Definition APPLY_sound := (@APPLY_sound _ (expr typ func) _ _ _ _ _ _ _ _ _ _ _ _ (fun (subst : Type)
+Check @APPLY_sound.
+Definition x: (ExprVar (expr typ func)) := _.
+Print x.
+
+Check APPLY_sound.
+(*Definition APPLY_sound := (@APPLY_sound _ (expr typ func) _ _ _ _ _ _ _ _ _ _ _ _ (fun (subst : Type)
                                  (SS : Subst subst (expr typ func))
                                  (SU : SubstUpdate subst (expr typ func))
                                  (tus tvs : tenv typ) 
@@ -59,9 +62,9 @@ Definition APPLY_sound := (@APPLY_sound _ (expr typ func) _ _ _ _ _ _ _ _ _ _ _ 
                                  RType_typ (func_defs.RSym_sym symexe.tbl)
                                  Typ2_tyArr SS SU
                                  (S (S (S (S (S (S (S (S (S (S O))))))))))
-                                 tus tvs n l r t3 s1) (ExprLift.vars_to_uvars_exprD')).
+                                 tus tvs n l r t3 s1) _ (* (ExprLift.vars_to_uvars_exprD')*)).*)
 
-Definition EAPPLY_sound := (@EAPPLY_sound _ (expr typ func) _ _ _ _ _ _ _ _ _ _ _ _ (fun (subst : Type)
+(*Definition EAPPLY_sound := (@EAPPLY_sound _ (expr typ func) _ _ _ _ _ _ _ _ _ _ _ _ (fun (subst : Type)
                                  (SS : Subst subst (expr typ func))
                                  (SU : SubstUpdate subst (expr typ func))
                                  (tus tvs : tenv typ) 
@@ -71,9 +74,10 @@ Definition EAPPLY_sound := (@EAPPLY_sound _ (expr typ func) _ _ _ _ _ _ _ _ _ _ 
                                  RType_typ (func_defs.RSym_sym symexe.tbl)
                                  Typ2_tyArr SS SU
                                  (S (S (S (S (S (S (S (S (S (S O))))))))))
-                                 tus tvs n l r t3 s1) (ExprLift.vars_to_uvars_exprD')).
+                                 tus tvs n l r t3 s1) (ExprLift.vars_to_uvars_exprD')).*)
 
-Lemma SYMEXE_STEP_SOUND : rtac_sound (Expr_expr := func_defs.Expr_expr_fs tbl) (SYMEXE_STEP).
+Lemma SYMEXE_STEP_sound : rtac_sound (Expr_expr := func_defs.Expr_expr_fs tbl) (SYMEXE_STEP tbl).
+Admitted. (*
 intros. eapply AT_GOAL_sound.
 intros. destruct (get_delta_statement e);
 repeat match goal with
@@ -81,7 +85,7 @@ repeat match goal with
            destruct X; try apply FAIL_sound
        end.
 + unfold APPLY_SKIP.
-  apply APPLY_sound. 
+  apply (@APPLY_sound typ (expr typ func)). 
   admit.
   - unfold skip_lemma. 
     unfold Lemma.lemmaD. simpl. intros. 
@@ -100,74 +104,160 @@ repeat match goal with
         simpl exprD'_typ0. simpl.
         unfold exprD'_typ0, ExprI.exprD'. simpl. erewrite exprD'_App_R_rw.
         2: reflexivity. 2: reflexivity.
-        Require Import get_set_reif_soundness.
-        Focus 2. eapply exprD'_App_L_rw; try reflexivity. 
-Admitted.
-(*
-        rewrite set_reif_eq2.
-        2: eapply exprD'_App_L_rw; [ reflexivity | reflexivity | eapply set_reif_eq2 ].
-
-
-        Opaque Traversable.mapT HList.hlist_app Lemma.foralls.
-        simpl.
-
-        destruct ( @exprD'_typ0 typ (expr typ func) RType_typ Expr_expr_fs Prop
-                 Typ0_tyProp (@nil typ)
-                 (@cons typ (tyArr tyenviron tympred)
-                    (@cons typ (typtree tyfunspec)
-                       (@cons typ (tylist tympred)
-                          (@cons typ tyOracleKind
-                             (@cons typ (typtree (typrod tyc_type tyval))
-                                (@cons typ (typtree tyval)
-                                   (@cons typ tyval (@nil typ))))))))
-                 (@App typ func
-                    (@App typ func
-                       (@Inj typ func
-                          (@inr
-                             (sum
-                                (sum SymEnv.func
-                                   (ModularFunc.ILogicFunc.ilfunc typ))
-                                (BILogicFunc.bilfunc typ)) func'
-                             (Other (feq (tyoption tyval)))))
-                       (set_reif.rmsubst_eval_expr
-                          (@Var typ func (S (S (S (S (S O))))))
-                          (@Var typ func (S (S (S (S O))))) e0))
-                    (@App typ func
-                       (@Inj typ func
-                          (@inr
-                             (sum
-                                (sum SymEnv.func
-                                   (ModularFunc.ILogicFunc.ilfunc typ))
-                                (BILogicFunc.bilfunc typ)) func'
-                             (Other (fsome tyval))))
-                       (@Var typ func (S (S (S (S (S (S O)))))))))) eqn:?. simpl.
-
-destruct (exprD'_typ0 []
-                   [tyArr tyenviron tympred; typtree tyfunspec;
-                   tylist tympred; tyOracleKind;
-                   typtree (typrod tyc_type tyval); 
-                   typtree tyval; tyval]
-                   (App
-                      (App
-                         (Inj (inr (Other (feq (tyArr tyenviron tympred)))))
-                         (App
-                            (App
-                               (App (Inj (inr (Smx fassertD)))
-                                  (Inj (inr (Data (..)))))
-                               (App
-                                  (App (Inj (inr (..)))
-                                     (get_set_reif.set_reif i 
-                                        (Var 6%nat) 
-                                        (Var 5%nat))) 
-                                  (Var 4%nat))) (Var 2%nat))) 
-                      (Var 0%nat))).
-  - 
-*)        
-
+(*        Focus 2. eapply exprD'_App_L_rw; try reflexivity.*) 
+Admitted. *)
 
 Lemma THEN'_sound : forall t1 t2, rtac_sound t1 -> rtac_sound t2 -> rtac_sound (THEN' t1 t2).
 intros. unfold THEN'. apply Then.THEN_sound. auto.
 apply runOnGoals_sound. auto.
 Qed.
 
+Theorem SYMEXE_sound : rtac_sound (SYMEXE_TAC tbl).
+unfold SYMEXE_TAC.
+apply THEN_sound.
+admit. (*jesper*)
+apply REPEAT_sound.
+apply SYMEXE_STEP_sound.
+Qed.
+
 End tbled.
+
+Require Import denote_tac.
+
+
+Ltac run_rtac reify term_table tac_sound :=
+  match type of tac_sound with
+    | forall t, @rtac_sound _ _ _ _ _ _ (?tac _) =>
+	  let name := fresh "e" in
+	  match goal with
+	    | |- ?P => 
+	      reify_aux reify term_table P name;
+              let tbl := get_tbl in
+	      let t := eval vm_compute in (@typeof_expr _ _ _ _ (RSym_sym tbl) nil nil name) in
+	      let goal := eval unfold name in name in
+	      match t with
+	        | Some ?t =>
+	          let goal_result := constr:(run_tac' (tac tbl) (GGoal name)) in 
+	          let result := eval vm_compute in goal_result in
+	          match result with
+	            | More_ ?s ?g => 
+	              cut (goalD_Prop nil nil g); [
+	                let goal_resultV := g in
+	               (* change (goalD_Prop nil nil goal_resultV -> exprD_Prop nil nil name);*)
+	                exact_no_check (@run_rtac_More tbl (tac tbl) _ _ _ (tac_sound tbl)
+	                	(@eq_refl (Result (CTop nil nil)) (More_ s goal_resultV) <:
+	                	   run_tac' (tac tbl) (GGoal goal) = (More_ s goal_resultV)))
+	                | cbv_denote
+	              ]
+	            | Solved ?s =>
+	              exact_no_check (@run_rtac_Solved tbl (tac tbl) s name (tac_sound tbl) 
+	                (@eq_refl (Result (CTop nil nil)) (Solved s) <: run_tac' (tac tbl) (GGoal goal) = Solved s))
+	            | Fail => idtac "Tactic" tac "failed."
+	            | _ => idtac "Error: run_rtac could not resolve the result from the tactic :" tac
+	          end
+	        | None => idtac "expression " goal "is ill typed" t
+	      end
+	  end
+	| _ => idtac tac_sound "is not a soudness theorem."
+  end.
+
+Ltac rforward := run_rtac reify_vst term_table SYMEXE_sound.
+
+
+Print Ltac run_rtac.
+Check run_tac'.
+
+Lemma skip_triple : forall p e,
+@semax e empty_tycontext
+     p
+      Sskip 
+     (normal_ret_assert p).
+Proof. 
+intros.
+unfold empty_tycontext.
+Time rforward.
+Qed.
+
+Fixpoint lots_of_skips n :=
+match n with 
+| O => Sskip
+| S n' => Ssequence Sskip (lots_of_skips n')
+end.
+
+Lemma seq_triple : forall p es,
+@semax es empty_tycontext p (Ssequence Sskip Sskip) (normal_ret_assert p).
+Proof.
+unfold empty_tycontext.
+rforward.
+Qed.
+
+Lemma seq_triple_lots : forall p es,
+@semax es empty_tycontext p (lots_of_skips 100) (normal_ret_assert p).
+Proof.
+unfold empty_tycontext.
+rforward.
+Qed.
+
+Require Import reverse_defs.
+Existing Instance NullExtension.Espec.
+
+Goal
+forall  (contents : list val), exists (PO : environ -> mpred), 
+   (semax
+     (remove_global_spec Delta) (*empty_tycontext*)
+     (assertD [] (localD (PTree.empty val) (PTree.empty (type * val))) [])
+     (Sset _p (Ecast (Econst_int (Int.repr 0) tint) (tptr tvoid)))         
+     (normal_ret_assert PO)).
+intros.
+unfold empty_tycontext, Delta, remove_global_spec. change PTree.tree with PTree.t.
+rforward.
+Qed.
+
+Goal
+forall  (contents : list val), exists PO, 
+   (semax
+     (remove_global_spec Delta)
+     (assertD [] (localD (PTree.empty val) (PTree.empty (type * val))) [])
+     (Ssequence (Sset _p (Ecast (Econst_int (Int.repr 0) tint) (tptr tvoid)))
+                Sskip)
+     (normal_ret_assert PO)).
+intros.
+unfold remove_global_spec,Delta.
+rforward.
+Qed.
+
+Fixpoint lots_temps' n p :=
+match n with 
+| O => PTree.set p (tptr t_struct_list, true) (PTree.empty _)
+| S n' =>  PTree.set p (tptr t_struct_list, true) (lots_temps' n' (Psucc p))
+end.
+
+Definition lots_temps (n : nat) : PTree.t (type * bool) := lots_temps' (S n) (1%positive).
+
+Fixpoint lots_of_sets' n p :=
+match n with 
+| O => (Sset p (Ecast (Econst_int (Int.repr 0) tint) (tptr tvoid)))
+| S n' => Ssequence (Sset p (Ecast (Econst_int (Int.repr 0) tint) (tptr tvoid))) (lots_of_sets' n' (Psucc p))
+end.
+
+Definition lots_of_sets n := lots_of_sets' n 1%positive.
+
+
+Goal
+forall  (contents : list val), exists PO, 
+   (semax
+     (mk_tycontext (lots_temps 50) (PTree.empty type) Tvoid
+     (PTree.empty type) (PTree.empty funspec))
+     (assertD [] (localD (PTree.empty val) (PTree.empty (type * val))) [])
+     (lots_of_sets 50)
+     (normal_ret_assert PO)).
+intros.
+unfold empty_tycontext, Delta, remove_global_spec. change PTree.tree with PTree.t.
+rforward.
+Qed.
+
+
+
+
+
+
